src/tls/MasterSecret.fst
@@ -1,0 +1,30 @@
+(* An experiment towards the PRF in KeySchedule, collapsing master and key derivation *)
+module MasterSecret (* : ST _ _ _ *)
+open FStar.HyperHeap
+
+(* tls_region is to be moved to TLSContants *)
+let tls_region = new_region root
+
+module AE = StreamAE
+module MM = MonotoneMap
+module MR = FStar.Monotonic.RRef
+
+let ms_tab : MM.t tls_region AE.id AE.writer (fun x -> True) =
+  MM.alloc #tls_region #AE.id #AE.writer #(fun x -> True)
+
+let derive (r:rid) (i:AE.id) 
+  : ST (AE.writer i)
+       (requires (fun h -> disjoint r tls_region))
+       (ensures (fun h0 w h1 -> 
+	   (* StreamAE.State.region w = r *) //not yet sure how to prove this part
+	   (* /\  *)modifies (Set.singleton tls_region) h0 h1
+	   /\ MR.witnessed (MM.t_contains ms_tab i w)))
+  = recall_region tls_region;
+    let y = MM.lookup ms_tab i in
+    match y with 
+    | None -> 
+      let w = AE.gen r i in 
+      MM.extend ms_tab i w;
+      w
+    | Some w -> 
+      w
